Dependency analysis to only reify  relevant hypotheses.
The solver collect dependencies. Yet, there is no correctness
proof (yet) and therefore they may be incomplete.
The information is only used to select hypotheses to reify.

src/cdcl.ml
@@ -378,9 +378,9 @@ let hcons i b f = P.HCons.{id = Uint63.of_int i; is_dec = b; elt = f}
 
 let reify_formula genv env k (f : EConstr.t) =
   let evd = env.Env.sigma in
-  let tt k = hcons 1 true (P.BForm.BTT k) in
-  let ff k = hcons 0 true (P.BForm.BFF k) in
-  let mkop k o f1 f2 = P.BForm.BOP (k, o, f1, f2) in
+  let tt k = hcons 1 true (P.BTT k) in
+  let ff k = hcons 0 true (P.BFF k) in
+  let mkop k o f1 f2 = P.BOP (k, o, f1, f2) in
   let eq_ind r i = GlobRef.equal r (GlobRef.IndRef i) in
   let eq_constructor r c = GlobRef.equal r (GlobRef.ConstructRef c) in
   let eq_const r c = GlobRef.equal r (GlobRef.ConstRef c) in
@@ -396,7 +396,7 @@ let reify_formula genv env k (f : EConstr.t) =
   let is_false = eq_constructor (Lazy.force coq_false) in
   let var env k f =
     let env', (atom, i) = Env.hcons_atom genv env k f in
-    (hcons i (Env.is_dec atom) (P.BForm.BAT (k, Uint63.of_int i)), env')
+    (hcons i (Env.is_dec atom) (P.BAT (k, Uint63.of_int i)), env')
   in
   let get_binop k t =
     match k with
@@ -452,8 +452,7 @@ let reify_formula genv env k (f : EConstr.t) =
         | Const (c, _) ->
           if is_is_True c then
             let f1, env = reify_formula env P.IsBool f1 in
-            ( hcons (Uint63.hash f1.P.HCons.id) true (P.BForm.BIT f1.P.HCons.elt)
-            , env )
+            (hcons (Uint63.hash f1.P.HCons.id) true (P.BIT f1.P.HCons.elt), env)
           else var env k f
         | _ -> var env k f ) )
     | _ -> var env k f
@@ -483,7 +482,7 @@ let make_formula env hyps hconcl =
       let hf2, env = make env hyps hconcl in
       let env, i = Env.hcons_op env P.IMPL hf1.P.HCons.id hf2.P.HCons.id in
       let is_dec = hf1.P.HCons.is_dec && hf2.P.HCons.is_dec in
-      (hcons i is_dec (P.BForm.BOP (P.IsProp, P.IMPL, hf1, hf2)), env)
+      (hcons i is_dec (P.BOP (P.IsProp, P.IMPL, hf1, hf2)), env)
   in
   make env hyps hconcl
 
@@ -567,7 +566,7 @@ let constr_of_bformula f =
   let mkop k o f1 f2 =
     EConstr.mkApp (mk_op, [|constr_of_kind k; constr_of_op o; f1; f2|])
   in
-  P.BForm.(
+  P.(
     let rec constr_of_op_formula f =
       match f with
       | BTT k -> tt k
@@ -873,6 +872,16 @@ let run_prover tac cc (genv, sigma) ep f =
 let fresh_id id gl =
   Tactics.fresh_id_in_env Id.Set.empty id (Proofview.Goal.env gl)
 
+let fresh_ids n id env =
+  let rec fresh n avoid acc =
+    if n = 0 then acc
+    else
+      let id = Names.Id.of_string (id ^ string_of_int n) in
+      let id = Tactics.fresh_id_in_env avoid id env in
+      fresh (n - 1) (Id.Set.add id avoid) (id :: acc)
+  in
+  fresh n Id.Set.empty []
+
 (* let clear_all_no_check =
   Proofview.Goal.enter (fun gl ->
       let concl = Tacmach.New.pf_concl gl in
@@ -900,44 +909,94 @@ let tclRETYPE c =
       let sigma, _ = Typing.type_of env sigma c in
       Unsafe.tclEVARS sigma)
 
-let assert_conflicts ep l gl =
-  let mk_goal c = Theory.constr_of_clause_dec ep c in
+let assert_conflicts l gl =
   let rec assert_conflicts n l =
     match l with
     | [] -> Tacticals.New.tclIDTAC
-    | (_, (c, prf)) :: l ->
-      let id = fresh_id (Names.Id.of_string ("__cc" ^ string_of_int n)) gl in
+    | (id, (c, prf)) :: l ->
       Tacticals.New.tclTHENLIST
-        [ Tactics.assert_by (Names.Name id) (mk_goal c)
+        [ Tactics.assert_by (Names.Name id) c
             (Tacticals.New.tclTHENLIST
                [(*Tactics.keep [];*) tclRETYPE prf; Tactics.exact_check prf])
-          (*    ; Tactics.generalize [EConstr.mkVar id] *)
         ; assert_conflicts (n + 1) l ]
   in
   assert_conflicts 0 l
 
-(** [assert_conflicts_clauses tac] runs the sat prover in ml 
+let rec output_list p o l =
+  match l with
+  | [] -> ()
+  | [e] -> p o e
+  | e :: l -> p o e; output_string o ";"; output_list p o l
+
+let output_pset o s =
+  ProverPatch.PSet.fold
+    (fun () k -> Printf.fprintf o "%i " (Uint63.hash k))
+    s ()
+
+let rec map_filter f l =
+  match l with
+  | [] -> []
+  | e :: l -> (
+    match f e with None -> map_filter f l | Some e' -> e' :: map_filter f l )
+
+(** [assert_conflict_clauses tac] runs the sat prover in ml 
     and asserts conflict_clauses *)
-let assert_conflicts_clauses tac =
+let collect_conflict_clauses tac gl =
+  let sigma = Tacmach.New.project gl in
+  let genv = Tacmach.New.pf_env gl in
+  let concl = Tacmach.New.pf_concl gl in
+  let hyps = Tacmach.New.pf_hyps_types gl in
+  let hyps, concl, env = reify_goal genv (Env.empty sigma) hyps concl in
+  if debug then
+    output_list
+      (fun o (h, f) ->
+        Printf.fprintf o "%s : %a\n" (Names.Id.to_string h)
+          ProverPatch.output_hbformula f)
+      stdout hyps;
+  let bform, env = make_formula env (List.rev hyps) concl in
+  let has_bool i =
+    try
+      let d = Env.AMap.find (Uint63.hash i) env.Env.amap in
+      Env.has_bool d
+    with Not_found -> false
+  in
+  let form = P.BForm.to_hformula has_bool bform in
+  let cc = ref [] in
+  match run_prover tac cc (genv, sigma) env form with
+  | P.Success ((hm, _cc), d) ->
+    let cc =
+      List.map
+        (fun (_, (c, prf)) -> (Theory.constr_of_clause_dec env c, prf))
+        !cc
+    in
+    let hyps =
+      map_filter
+        (fun (h, f) -> if P.PSet.mem f.P.HCons.id d then Some h else None)
+        hyps
+    in
+    if debug then (
+      Printf.printf "Deps %a\n" output_pset d;
+      Printf.printf "Hyps %a\n"
+        (output_list (fun o h -> output_string o (Names.Id.to_string h)))
+        hyps );
+    Some (cc, hyps)
+  | _ -> None
+
+let assert_conflict_clauses tac =
   Proofview.Goal.enter (fun gl ->
       Coqlib.check_required_library ["Cdcl"; "Formula"];
-      let sigma = Tacmach.New.project gl in
-      let genv = Tacmach.New.pf_env gl in
-      let concl = Tacmach.New.pf_concl gl in
-      let hyps = Tacmach.New.pf_hyps_types gl in
-      let hyps, concl, env = reify_goal genv (Env.empty sigma) hyps concl in
-      let bform, env = make_formula env (List.rev hyps) concl in
-      let has_bool i =
-        try
-          let d = Env.AMap.find (Uint63.hash i) env.Env.amap in
-          Env.has_bool d
-        with Not_found -> false
-      in
-      let form = P.BForm.to_hformula has_bool bform in
-      let cc = ref [] in
-      match run_prover tac cc (genv, sigma) env form with
-      | P.HasProof _ -> assert_conflicts env !cc gl
-      | _ -> Tacticals.New.tclFAIL 0 (Pp.str "Not a tautology"))
+      match collect_conflict_clauses tac gl with
+      | None -> Tacticals.New.tclFAIL 0 (Pp.str "Not a tautology")
+      | Some (cc, d) ->
+        let ids = fresh_ids (List.length cc) "__cc" (Proofview.Goal.env gl) in
+        let cc = List.combine ids cc in
+        Tacticals.New.tclTHENLIST
+          [ (* Assert the conflict clauses *)
+            assert_conflicts cc gl
+          ; (* Generalize the used hypotheses *)
+            Tactics.generalize (List.map EConstr.mkVar d)
+          ; (* Generalize the conflict clauses *)
+            Tactics.generalize (List.map EConstr.mkVar ids) ])
 
 let generalize_prop =
   Proofview.Goal.enter (fun gl ->
@@ -947,7 +1006,6 @@ let generalize_prop =
       let hyps = List.filter (fun (_, t) -> is_prop genv sigma t) hyps in
       Tactics.generalize (List.map (fun x -> EConstr.mkVar (fst x)) hyps))
 
-(* I have no idea what [tclWITHHOLES] does but it fails (rightly) more often than [generalize] alone. *)
 let feedback msg =
   Proofview.Goal.enter (fun gl ->
       Feedback.msg_debug msg; Tacticals.New.tclIDTAC)
@@ -1014,7 +1072,3 @@ let nnpp =
       if is_loaded_library ["Coq"; "Logic"; "Classical_Prop"] then
         Tactics.apply (Lazy.force coq_nnpp)
       else Tacticals.New.tclIDTAC)
-
-let cdcl tac =
-  Tacticals.New.tclTHENLIST
-    [generalize_prop; assert_conflicts_clauses tac; change_goal]
